LogicalRefinement/Typed/Wk.lean
@@ -99,6 +99,8 @@ theorem HasType.wk {Δ a A} (HΔ: Δ ⊢ a: A):
       apply HasVar.wk
       repeat assumption
 
+    case funext => sorry
+
     all_goals (
       intro ρ Γ R;
       rename_i' I5 I4 I3 I2 I1 I0;
